open import Agda.Primitive
open import Relation.Unary hiding (_âˆˆ_)
open import Relation.Binary
open import Relation.Binary.PropositionalEquality
open import Data.Product using (_,_)
open import Function using (_âˆ˜_)

open â‰¡-Reasoning

import Syntax
import Renaming


module Substitution (Class : Set) where

  open Syntax Class
  open Renaming Class

  -- Lifting of renamings to substitutions, and of variables to expressions

  lift : âˆ€ {Î³ Î´} â†’ (Î³ â†’Ê³ Î´) â†’ (Î³ â†’Ë¢ Î´)

  Î· : âˆ€ {Î³ a} (x : a âˆˆ Î³) â†’ Arg Î³ a

  lift ğŸ˜ = ğŸ˜
  lift [ x ] = [ Î· x ]
  lift (Ïâ‚ âŠ• Ïâ‚‚) = lift Ïâ‚ âŠ• lift Ïâ‚‚

  Î· x = var-left x ` lift (tabulate var-right)

  -- Ideally we would like the following to be the definition of lift,
  -- but Agda termination gets in the way

  lift-map-Î· : âˆ€ {Î³ Î´} (Ï : Î³ â†’Ê³ Î´) â†’ lift Ï â‰¡ map Î· Ï
  lift-map-Î· ğŸ˜ = refl
  lift-map-Î· [ x ] = refl
  lift-map-Î· (Ïâ‚ âŠ• Ïâ‚‚) = congâ‚‚ _âŠ•_ (lift-map-Î· Ïâ‚) (lift-map-Î· Ïâ‚‚)

  lift-ğŸ™Ê³ : âˆ€ {Î³} â†’ lift ğŸ™Ê³ â‰¡ tabulate (Î· {Î³ = Î³})
  lift-ğŸ™Ê³ = trans (lift-map-Î· ğŸ™Ê³) map-tabulate

  -- Identity substitution

  ğŸ™Ë¢ : âˆ€ {Î³} â†’ Î³ â†’Ë¢ Î³
  ğŸ™Ë¢ = lift ğŸ™Ê³

  -- Substitution extension

  â‡‘Ë¢ : âˆ€ {Î³ Î´ Î¸} â†’ Î³ â†’Ë¢ Î´ â†’ Î³ âŠ• Î¸ â†’Ë¢ Î´ âŠ• Î¸
  â‡‘Ë¢ {Î¸ = Î¸} f =  map [ â‡‘Ê³ (tabulate var-left) ]Ê³_ f âŠ• lift (tabulate var-right)

  -- The interaction of lifting with various operations

  lift-âˆ™ : âˆ€ {Î³ Î´} (Ï : Î³ â†’Ê³ Î´) {a} (x : a âˆˆ Î³) â†’
           lift Ï âˆ™ x â‰¡ Î· (Ï âˆ™ x)
  lift-âˆ™ [ _ ] var-here = refl
  lift-âˆ™ (Ïâ‚ âŠ• Ïâ‚‚) (var-left x) = lift-âˆ™ Ïâ‚ x
  lift-âˆ™ (Ïâ‚ âŠ• Ïâ‚‚) (var-right y) = lift-âˆ™ Ïâ‚‚ y

  lift-tabulate : âˆ€ {Î³ Î´} (f : âˆ€ {Î±} â†’ Î± âˆˆ Î³ â†’ Î± âˆˆ Î´) {a} (x : a âˆˆ Î³) â†’
                  lift (tabulate f) âˆ™ x â‰¡ Î· (f x)
  lift-tabulate f var-here = refl
  lift-tabulate f (var-left x) = lift-tabulate (Î» z â†’ f (var-left z)) x
  lift-tabulate f (var-right y) = lift-tabulate (Î» z â†’ f (var-right z)) y

  âˆ˜Ê³-lift : âˆ€ {Î³ Î´ Î¸} (Ï : Î³ â†’Ê³ Î´) (Ï„ : Î´ â†’Ê³ Î¸) {a} (x : a âˆˆ Î³) â†’
             lift (Ï„ âˆ˜Ê³ Ï) âˆ™ x â‰¡  lift Ï„ âˆ™ (Ï âˆ™ x)
  âˆ˜Ê³-lift [ x ] Ï„ var-here = sym (lift-âˆ™ Ï„ x)
  âˆ˜Ê³-lift (Ïâ‚ âŠ• Ïâ‚‚) Ï„ (var-left x) = âˆ˜Ê³-lift Ïâ‚ Ï„ x
  âˆ˜Ê³-lift (Ïâ‚ âŠ• Ïâ‚‚) Ï„ (var-right y) = âˆ˜Ê³-lift Ïâ‚‚ Ï„ y

  []Ê³-lift : âˆ€ {Î³ Î´ Î¸} (Ï : Î³ â†’Ê³ Î´) (Ï„ : Î´ â†’Ê³ Î¸) {a} (x : a âˆˆ Î³) â†’ [ â‡‘Ê³ Ï„ ]Ê³ (lift Ï âˆ™ x) â‰¡  lift (Ï„ âˆ˜Ê³ Ï) âˆ™ x
  []Ê³-Î· : âˆ€ {Î³ Î´} (Ï : Î³ â†’Ê³ Î´) {a} (x : a âˆˆ Î³) â†’ [ â‡‘Ê³ Ï ]Ê³ Î· x â‰¡ Î· (Ï âˆ™ x)

  []Ê³-lift [ x ] Ï„ var-here = []Ê³-Î· Ï„ x
  []Ê³-lift (Ïâ‚ âŠ• Ïâ‚‚) Ï„ (var-left x) = []Ê³-lift Ïâ‚ Ï„ x
  []Ê³-lift (Ïâ‚ âŠ• Ïâ‚‚) Ï„ (var-right x) = []Ê³-lift Ïâ‚‚ Ï„ x

  â‡‘Ê³-âˆ˜Ê³-tabulate-var-right : âˆ€ {Î³ Î´ Î¸} (Ï : Î³ â†’Ê³ Î´) â†’
                             (â‡‘Ê³ {Î¸ = Î¸} Ï âˆ˜Ê³ tabulate var-right) â‰¡ tabulate var-right
  â‡‘Ê³-âˆ˜Ê³-tabulate-var-right {Î¸ = Î¸} Ï = shape-â‰¡ Î¾
    where Î¾ : âˆ€ {a} (x : a âˆˆ Î¸) â†’ (â‡‘Ê³ Ï âˆ˜Ê³ tabulate var-right) âˆ™ x â‰¡ tabulate var-right âˆ™ x
          Î¾ x = trans
                  (trans
                      (âˆ˜Ê³-âˆ™  {Ï = â‡‘Ê³ Ï} {Ï„ = tabulate var-right} {x = x})
                      (trans (cong (â‡‘Ê³ Ï âˆ™_) (tabulate-âˆ™ var-right)) (tabulate-âˆ™ var-right)))
                  (sym (tabulate-âˆ™ var-right))

  [â‡‘Ê³]-lift-var-right : âˆ€ {Î³ Î´ Î¸} (Ï : Î³ â†’Ê³ Î´) {a} (x : a âˆˆ Î¸) â†’
                        [ â‡‘Ê³ (â‡‘Ê³ Ï) ]Ê³ lift (tabulate var-right) âˆ™ x  â‰¡ lift (tabulate var-right) âˆ™ x
  [â‡‘Ê³]-lift-var-right Ï x = trans ([]Ê³-lift (tabulate var-right) (â‡‘Ê³ Ï) x) (cong (Î» Ï„ â†’ lift Ï„ âˆ™ x) (â‡‘Ê³-âˆ˜Ê³-tabulate-var-right Ï))

  Ê³âˆ˜Ë¢-lift-var-right : âˆ€ {Î³ Î´ Î¸} (Ï : Î³ â†’Ê³ Î´) {a} (x : a âˆˆ Î¸) â†’
                       ((â‡‘Ê³ {Î¸ = Î¸} Ï) Ê³âˆ˜Ë¢ lift (tabulate var-right)) âˆ™ x â‰¡ lift (tabulate var-right) âˆ™ x
  Ê³âˆ˜Ë¢-lift-var-right Ï x =
    trans
      (Ê³âˆ˜Ë¢-âˆ™ {Ï = â‡‘Ê³ Ï} {ts = lift (tabulate var-right)})
      ([â‡‘Ê³]-lift-var-right Ï x)

  []Ê³-Î· Ï x = â‰¡-` (map-âˆ™ {f = var-left} {ps = Ï}) (Î» z â†’ Ê³âˆ˜Ë¢-lift-var-right Ï z)


  Ê³âˆ˜Ë¢-lift : âˆ€ {Î³ Î´ Î¸} (Ï : Î³ â†’Ê³ Î´) (Ï„ : Î´ â†’Ê³ Î¸) {a} (x : a âˆˆ Î³) â†’
             (Ï„ Ê³âˆ˜Ë¢ lift Ï) âˆ™ x â‰¡ lift (Ï„ âˆ˜Ê³ Ï) âˆ™ x
  Ê³âˆ˜Ë¢-lift [ x ] Ï„ var-here = â‰¡-` ( map-âˆ™ {f = var-left} {ps = Ï„}) Î» z â†’ Ê³âˆ˜Ë¢-lift-var-right Ï„ z
  Ê³âˆ˜Ë¢-lift (Ïâ‚ âŠ• Ïâ‚‚) Ï„ (var-left x) = Ê³âˆ˜Ë¢-lift Ïâ‚ Ï„ x
  Ê³âˆ˜Ë¢-lift (Ïâ‚ âŠ• Ïâ‚‚) Ï„ (var-right x) = Ê³âˆ˜Ë¢-lift Ïâ‚‚ Ï„ x

  lift-map : âˆ€ {Î³ Î´ Î¸} (f : âˆ€ {Î±} â†’ Î± âˆˆ Î³ â†’ Î± âˆˆ Î´) (Ï : Î¸ â†’Ê³ Î³) â†’
             lift (map f Ï) â‰¡ map [ â‡‘Ê³ (tabulate f) ]Ê³_ (lift Ï)
  lift-map f ğŸ˜ = refl
  lift-map f [ x ] = cong [_] (trans (cong Î· (sym (tabulate-âˆ™ f))) (sym ([]Ê³-Î· (tabulate f) x)))
  lift-map f (Ïâ‚ âŠ• Ïâ‚‚) = congâ‚‚ _âŠ•_ (lift-map f Ïâ‚) (lift-map f Ïâ‚‚)

  â‡‘Ë¢-lift : âˆ€ {Î³ Î´ Î¸} (Ï : Î³ â†’Ê³ Î´) â†’ â‡‘Ë¢ {Î¸ = Î¸} (lift Ï) â‰¡ lift (â‡‘Ê³ Ï)
  â‡‘Ë¢-lift Ï = congâ‚‚ _âŠ•_ (sym (lift-map var-left Ï)) refl


  -- Action of substitution
  infix 6 [_]Ë¢_
  infix 6 _âˆ˜Ë¢_

  -- -- The naive definition, which Agda does not see as terminating
  -- [_]Ë¢_ : âˆ€ {Î³ Î´ cl} (f : Î³ â†’Ë¢ Î´) â†’ Expr Î³ cl â†’ Expr Î´ cl
  -- _âˆ˜Ë¢_ : âˆ€ {Î³ Î´ Î¸} (g : Î´ â†’Ë¢ Î¸) (f : Î³ â†’Ë¢ Î´) â†’ Î³ â†’Ë¢ Î¸
  -- [ f ]Ë¢ x ` ts = [ ğŸ™Ë¢ âŠ• (f âˆ˜Ë¢ ts) ]Ë¢ (f âˆ™ x)
  -- g âˆ˜Ë¢ f = tabulate (Î» x â†’ [ â‡‘Ë¢ g ]Ë¢ f âˆ™ x)

  -- Instead we use the Bove-Cappreta method, whereby we define the support of [_]Ë¢_ and _âˆ˜Ë¢_, then we define the maps
  -- as partial maps defined on the support, and finally show that the supports are the entire domains.
  -- See doi:10.1017/S0960129505004822

  data defined-[]Ë¢ : âˆ€ {Î³ Î´ cl} (f : Î³ â†’Ë¢ Î´) â†’ Expr Î³ cl â†’ Set

  data defined-âˆ˜Ë¢ : âˆ€ {Î³ Î´ Î¸} (g : Î´ â†’Ë¢ Î¸) (f : Î³ â†’Ë¢ Î´) â†’ Set

  actË¢ : âˆ€ {Î³ Î´ cl} (f : Î³ â†’Ë¢ Î´) (e : Expr Î³ cl) â†’ defined-[]Ë¢ f e â†’ Expr Î´ cl

  compË¢ : âˆ€ {Î³ Î´ Î¸} (g : Î´ â†’Ë¢ Î¸) (f : Î³ â†’Ë¢ Î´) â†’ defined-âˆ˜Ë¢ g f â†’ (Î³ â†’Ë¢ Î¸)

  data defined-[]Ë¢ where
    def-[]Ë¢ : âˆ€ {Î³ Î³' Î´ cl} {f : Î³ â†’Ë¢ Î´} {x : (Î³' , cl) âˆˆ Î³} {ts : Î³' â†’Ë¢ Î³} (D : defined-âˆ˜Ë¢ f ts) â†’
              defined-[]Ë¢ (ğŸ™Ë¢ âŠ• (compË¢ f ts D)) (f âˆ™ x) â†’
              defined-[]Ë¢ f (x ` ts)

  data defined-âˆ˜Ë¢ where
    def-âˆ˜Ë¢ :  âˆ€ {Î³ Î´ Î¸} {g : Î´ â†’Ë¢ Î¸} {f : Î³ â†’Ë¢ Î´} â†’
              (âˆ€ {Î³' cl} (x : (Î³' , cl) âˆˆ Î³) â†’ defined-[]Ë¢ (â‡‘Ë¢ g) (f âˆ™ x)) â†’ defined-âˆ˜Ë¢ g f

  actË¢ f (x ` ts) (def-[]Ë¢ D E) = actË¢ (ğŸ™Ë¢ âŠ• (compË¢ f ts D)) (f âˆ™ x) E

  compË¢ g f (def-âˆ˜Ë¢ D) = tabulate (Î» x â†’ actË¢ (â‡‘Ë¢ g) (f âˆ™ x) (D x))

  -- Showing that actË¢ and compË¢ are total requires several steps.

  is-total-[]Ë¢ : âˆ€ {Î³ Î´} (f : Î³ â†’Ë¢ Î´) â†’ Set
  is-total-[]Ë¢ {Î³ = Î³} f = âˆ€ {cl} (e : Expr Î³ cl) â†’ defined-[]Ë¢ f e

  âŠ•-total-[]Ë¢ : âˆ€ {Î³ Î´ Î¸} {f : Î³ â†’Ë¢ Î¸} {g : Î´ â†’Ë¢ Î¸} â†’ is-total-[]Ë¢ f â†’ is-total-[]Ë¢ g â†’ is-total-[]Ë¢ (f âŠ• g)

  âŠ•-total-âˆ˜Ë¢ : âˆ€ {Ï‡ Î³ Î´ Î¸} {h : Ï‡ â†’Ë¢ Î³ âŠ• Î´} {f : Î³ â†’Ë¢ Î¸} {g : Î´ â†’Ë¢ Î¸} â†’
                 is-total-[]Ë¢ f â†’ is-total-[]Ë¢ g â†’ is-total-[]Ë¢ h â†’ defined-âˆ˜Ë¢ (f âŠ• g) h

  âŠ•-total-[]Ë¢ ft gt (var-left x ` ts) = def-[]Ë¢ (âŠ•-total-âˆ˜Ë¢ ft gt {!!}) {!!}
  âŠ•-total-[]Ë¢ ft gt (var-right y ` ts) = {!!}

  âŠ•-total-âˆ˜Ë¢ ft gt ht = {!!}

  []Ë¢-lift-total : âˆ€ {Î³ Î´ cl} (Ï : Î³ â†’Ê³ Î´) (e : Expr Î³ cl) â†’ defined-[]Ë¢ (lift Ï) e
  []Ë¢-lift-total Ï (x ` ts) =
    def-[]Ë¢
      (def-âˆ˜Ë¢ (Î» y â†’ subst (Î» Ï„ â†’ defined-[]Ë¢ Ï„ (ts âˆ™ y)) (sym (â‡‘Ë¢-lift Ï)) {!!}))
      {!!}


  -- The identity substitution is total
  []-ğŸ™Ë¢-total : âˆ€ {Î³ cl} (e : Expr Î³ cl) â†’ defined-[]Ë¢ ğŸ™Ë¢ e
  []-ğŸ™Ë¢-total (x ` ts) = def-[]Ë¢ (def-âˆ˜Ë¢ (Î» y â†’ {!!})) {!!}


  total-actË¢ : âˆ€ {Î³ Î´ cl} (f : Î³ â†’Ë¢ Î´) (e : Expr Î³ cl) â†’ defined-[]Ë¢ f e
  total-compË¢ : âˆ€ {Î³ Î´ Î¸} (g : Î´ â†’Ë¢ Î¸) (f : Î³ â†’Ë¢ Î´) â†’ defined-âˆ˜Ë¢ g f

  total-actË¢ f (x ` ts) = def-[]Ë¢ (total-compË¢ f ts) {!!}

  total-compË¢ {Î³ = Î³} f g = def-âˆ˜Ë¢ Î» {Î³' cl} (x : (Î³' , cl) âˆˆ Î³) â†’ {!!}


  -- Finally, the definitions we wanted to get

  [_]Ë¢_ : âˆ€ {Î³ Î´ cl} (f : Î³ â†’Ë¢ Î´) â†’ Expr Î³ cl â†’ Expr Î´ cl
  [ f ]Ë¢ e = actË¢ f e (total-actË¢ f e)

  _âˆ˜Ë¢_ : âˆ€ {Î³ Î´ Î¸} (g : Î´ â†’Ë¢ Î¸) (f : Î³ â†’Ë¢ Î´) â†’ Î³ â†’Ë¢ Î¸
  g âˆ˜Ë¢ f = compË¢ g f (total-compË¢ g f)
